first attempts at freeze

src/Arithmetic/Saturated.v
@@ -8,6 +8,7 @@ Require Import Crypto.Arithmetic.Core.
 Require Import Crypto.Util.LetIn Crypto.Util.CPSUtil.
 Require Import Crypto.Util.Tuple Crypto.Util.ListUtil.
 Require Import Crypto.Util.Tactics.BreakMatch.
+Require Import Crypto.Util.Decidable Crypto.Util.ZUtil.
 Local Notation "A ^ n" := (tuple A n) : type_scope.
 
 (***
@@ -101,7 +102,7 @@ check confirms our result.
 
 Module Columns.
   Section Columns.
-    Context {weight : nat->Z}
+    Context (weight : nat->Z)
             {weight_0 : weight 0%nat = 1}
             {weight_nonzero : forall i, weight i <> 0}
             {weight_multiples : forall i, weight (S i) mod weight i = 0}
@@ -231,12 +232,12 @@ Module Columns.
     Qed.
 
     Lemma eval_compact {n} (xs : tuple (list Z) n) :
-      B.Positional.eval weight (snd (compact xs)) + (weight n * fst (compact xs)) = eval xs.
+      B.Positional.eval weight (snd (compact xs)) = eval xs - (weight n * fst (compact xs)).
     Proof using Type*.
       pose proof (compact_invariant_end 0 xs) as Hinv.
       cbv [compact_invariant] in Hinv.
       simpl in Hinv. autorewrite with zsimplify natsimplify in Hinv.
-      rewrite eval_from_0, B.Positional.eval_from_0 in Hinv; apply Hinv.
+      rewrite eval_from_0, B.Positional.eval_from_0 in Hinv. nsatz.
     Qed.
 
     Definition cons_to_nth_cps {n} i (x:Z) (t:(list Z)^n)
@@ -339,9 +340,223 @@ Module Columns.
         (fun P => B.Positional.to_associational_cps weight q
         (fun Q => from_associational_cps n (P++Q) f)).
 
+    Definition sub_cps {n} (p q : Z^n) {T} (f : (list Z)^n->T) :=
+      B.Positional.to_associational_cps weight p
+        (fun P => B.Positional.to_associational_cps weight q
+        (fun Q => from_associational_cps n (P++Q) f)).
+
   End Columns.
 End Columns.
+Hint Unfold
+     Columns.add_cps
+     Columns.mul_cps
+     Columns.sub_cps.
+Hint Rewrite
+     @Columns.compact_digit_id
+     @Columns.compact_step_id
+     @Columns.compact_id
+     @Columns.cons_to_nth_id
+     @Columns.from_associational_id
+  : uncps.
+Hint Rewrite
+     @Columns.eval_compact
+     @Columns.eval_cons_to_nth
+     @Columns.eval_from_associational
+     @Columns.eval_nils
+  using (assumption || omega): push_basesystem_eval.
 
+Section Freeze.
+  Context (weight : nat->Z)
+          {weight_0 : weight 0%nat = 1}
+          {weight_nonzero : forall i, weight i <> 0}
+          {weight_multiples : forall i, weight (S i) mod weight i = 0}
+          (* add_get_carry takes in a number at which to split output *)
+          {add_get_carry: Z ->Z -> Z -> (Z * Z)}
+          {add_get_carry_correct : forall s x y,
+              fst (add_get_carry s x y)  = x + y - s * snd (add_get_carry s x y)}
+  .
+
+  (* adds p and q if cond is 0, else adds 0 to p*)
+  Definition conditional_mask_cps {n} (mask:Z) (cond:Z) (p:Z^n)
+             {T} (f:_->T) :=
+    dlet and_term := if (dec (cond = 0)) then 0 else mask in
+    f (Tuple.map (Z.land and_term) p).
+
+  Definition conditional_mask {n} mask cond p :=
+    @conditional_mask_cps n mask cond p _ id.
+  Lemma conditional_mask_id {n} mask cond p T f:
+    @conditional_mask_cps n mask cond p T f
+    = f (conditional_mask mask cond p).
+  Proof.
+    cbv [conditional_mask_cps conditional_mask Let_In]; break_match;
+      autounfold; autorewrite with uncps push_id; reflexivity.
+  Qed.
+  Hint Opaque conditional_mask : uncps.
+  Hint Rewrite @conditional_mask_id : uncps.
+
+  Definition conditional_add_cps {n} mask cond (p q : Z^n) {T} (f:_->T) :=
+    conditional_mask_cps mask cond q
+    (fun qq => Columns.add_cps weight p qq
+    (fun R => Columns.compact_cps (add_get_carry:=add_get_carry) weight R f)).
+  Definition conditional_add {n} mask cond p q :=
+    @conditional_add_cps n mask cond p q _ id.
+  Lemma conditional_add_id {n} mask cond p q T f:
+    @conditional_add_cps n mask cond p q T f
+    = f (conditional_add mask cond p q).
+  Proof.
+    cbv [conditional_add_cps conditional_add]; autounfold;
+      autorewrite with uncps push_id; reflexivity.
+  Qed.
+  Hint Opaque conditional_add : uncps.
+  Hint Rewrite @conditional_add_id : uncps.
+  
+  
+  (*
+    [freeze] has the following steps:
+    (1) pseudomersenne reduction using [carry_reduce]
+    (2) subtract modulus in a carrying loop (in our framework, this
+    consists of two steps; [Columns.sub_cps] combines the input p and
+    the modulus m such that the ith limb in the output is the list
+    [p[i];-m[i]]. We can then call [Columns.compact].)
+    (3) look at the final carry, which should be either 0 or -1. If
+    it's -1, then we add the modulus back in. Otherwise we add 0 for
+    constant-timeness.
+    (4) discard the carry after this last addition; it should be 1 if
+    the carry in step 3 was -1, so they cancel out.
+   *)
+  Definition freeze_cps
+             {n} (mask:Z) (s:Z) (c:list B.limb) (m:Z^n) (p:Z^n)
+             {T} (f : Z^n->T) :=
+    B.Positional.carry_reduce_cps
+      (div:=div) (modulo:=modulo) weight s c p
+      (fun P => Columns.sub_cps weight P m
+      (fun Q => Columns.compact_cps (add_get_carry:=add_get_carry) weight Q
+      (fun carry_q => conditional_add_cps mask (fst carry_q) (snd carry_q) m
+      (fun carry_r => f (snd carry_r)))))
+  .
+
+  SearchAbout (((_ mod _) mod _)).
+
+  Definition freeze {n} mask s c m p :=
+    @freeze_cps n mask s c m p _ id.
+  Lemma freeze_id {n} mask s c m p T f:
+    @freeze_cps n mask s c m p T f = f (freeze mask s c m p).
+  Proof.
+    cbv [freeze_cps freeze]; repeat progress autounfold;
+      autorewrite with uncps push_id; reflexivity.
+  Qed.
+  Hint Opaque freeze : uncps.
+  Hint Rewrite @freeze_id : uncps.
+
+  Lemma map_land_zero {n} (p:Z^n):
+    Tuple.map (Z.land 0) p = B.Positional.zeros n.
+  Proof.
+    induction n; [ destruct p; reflexivity | ].
+    replace p with (append (hd p) (tl p)) by
+        (simpl in p; destruct n; destruct p; reflexivity).
+    rewrite map_append, IHn, Z.land_0_l; reflexivity.
+  Qed.
+
+  Lemma eval_conditional_mask {n} mask cond p (n_nonzero:n<>0%nat)
+    (Hmask : Tuple.map (Z.land mask) p = p):
+    B.Positional.eval weight (@conditional_mask n mask cond p)
+    = if (dec (cond = 0)) then 0 else B.Positional.eval weight p.
+  Proof.
+    cbv [conditional_mask_cps conditional_mask Let_In];
+      repeat progress autounfold; break_match;
+        rewrite ?Hmask, ?map_land_zero;
+        autorewrite with uncps push_id push_basesystem_eval; ring.
+  Qed.
+  Hint Rewrite @eval_conditional_mask using (omega || assumption)
+    : push_basesystem_eval.
+
+  Lemma eval_conditional_add {n} mask cond p q (n_nonzero:n<>0%nat)
+    (Hmask : Tuple.map (Z.land mask) q = q):
+    B.Positional.eval weight (snd (@conditional_add n mask cond p q))
+    = B.Positional.eval weight p + (if (dec (cond = 0)) then 0 else B.Positional.eval weight q) - weight n * (fst (conditional_add mask cond p q)).
+  Proof.
+    cbv [conditional_add_cps conditional_add];
+      repeat progress autounfold; rewrite ?Hmask, ?map_land_zero; 
+        autorewrite with uncps push_id push_basesystem_eval;
+        break_match; ring.
+  Qed.
+  Hint Rewrite @eval_conditional_add using (omega || assumption)
+    : push_basesystem_eval.
+
+  Lemma freezeZ m s c y0 z z0 c0 a :
+    m = s - c ->
+    0 < c < s ->
+    s <> 0 ->
+    -m <= y0 < m ->
+    z = y0 mod s ->
+    c0 = y0 / s ->
+    c0 <> 0 ->
+    z0 = z + m ->
+    a = z0 mod s ->
+    a mod m = y0 mod m.
+  Proof.
+    clear. intros. subst.
+    rewrite Z.add_mod by assumption.
+    rewrite Z.mod_mod by assumption.
+    rewrite <-Z.add_mod by assumption.
+    assert (~ (0 <= y0 < s)) by (pose proof (Z.div_small y0 s); tauto).
+    assert (-(s-c) <= y0 < 0) by omega.
+    rewrite Z.mod_small with (b := s) by omega.
+    rewrite Z.add_mod, Z.mod_same, Z.add_0_r, Z.mod_mod by omega.
+    reflexivity.
+  Qed.
+
+  Lemma eval_freeze {n} mask s c m p
+        (n_nonzero:n<>0%nat) (s_nonzero:s<>0)
+        (Hweight : weight (S (pred n)) / weight (pred n) <> 0)
+        (Hmask : Tuple.map (Z.land mask) m = m)
+        modulus (Hm : B.Positional.eval weight m = Z.pos modulus)
+        (Hsc : Z.pos modulus = s - B.Associational.eval c)
+    :
+      mod_eq modulus
+             (B.Positional.eval weight (@freeze n mask s c m p))
+             (B.Positional.eval weight p).
+  Proof.
+    cbv [freeze_cps freeze mod_eq]; repeat progress autounfold;
+      autorewrite with uncps push_id.
+    
+    assert (Z.pos modulus <> 0) by (pose proof Pos2Z.is_pos modulus; omega).
+    pose proof div_mod.
+    break_match; subst.
+    
+    rewrite Z.mul_0_r, Z.add_0_r, Z.sub_0_r.
+    (* TODO : how to prove second carry is 0? *)
+    rewrite Z.add_mod, B.Associational.eval_reduce by assumption.
+    autorewrite with uncps push_id push_basesystem_eval.
+    rewrite Hm. autorewrite with zsimplify.
+    reflexivity.
+
+    
+    ring_simplify.
+    let p := fresh "P" in
+    let carry := fresh "carry" in
+    let result := fresh "result" in
+    match goal with H:fst ?x <> 0 |- _ =>
+                         remember x as p; destruct p as [carry result];
+                           autorewrite with cancel_pair in *
+    end.
+    rewrite Columns.eval_from_associational by assumption.
+    autorewrite with uncps push_id push_basesystem_eval.
+    rewrite Hm.
+    Check Z.add_mod_full.
+    match goal with |- context [(?a + ?b - ?c + ?d) mod ?m] =>
+                    replace (a + b - c + d) with (b + (a-c) + d) by ring;
+                    rewrite (Z.add_mod_full _ d), (Z.add_mod_full _ (a-c))
+    end.
+    rewrite !Z.mod_same by assumption.
+    rewrite !Z.add_0_r, !Z.add_0_l.
+    rewrite !Z.mod_mod by assumption.
+    rewrite Z.sub_mod_full.
+    rewrite B.Associational.eval_reduce by assumption.
+    autorewrite with uncps push_id push_basesystem_eval.
+    
+
+  
 (*
 (* Just some pretty-printing *)
 Local Notation "fst~ a" := (let (x,_) := a in x) (at level 40, only printing).
